src/program_proof/session/processRequest.v
@@ -213,10 +213,10 @@ Section heap.
         ⌜SERVER_INVARIANT (fun _s => True) (coq_processRequest s msg).1⌝
     }}}.
   Proof.
-    (* unfold is_server. rewrite redefine_server_val redefine_message_val. TypeVector.des sv. TypeVector.des msgv. iIntros "%Φ (H_server & H_message & %H_precondition) HΦ".
+    unfold is_server. rewrite redefine_server_val redefine_message_val. TypeVector.des sv. TypeVector.des msgv. iIntros "%Φ (H_server & H_message & %H_precondition) HΦ".
     iDestruct "H_server" as "(%H1 & %H2 & H3 & H4 & %H5 & H6 & H7 & H8 & H9 & %H10)".
     iDestruct "H_message" as "(%H11 & %H12 & %H13 & %H14 & %H15 & H16 & %H17 & %H18 & %H19 & H20 & %H21 & %H22 & %H23 & %H24 & %H25 & %H26 & H27 & %H28 & %H29 & %H30)".
-    destruct H_precondition as [? ? ? ?]; simplNotation; subst; rewrite /CoqSessionServer.processRequest.
+    destruct H_precondition as [? ? ? ? ?]; simplNotation; subst; rewrite /CoqSessionServer.processRequest. repeat match goal with [ H : ?x = _ /\ _ |- _ ] => let x' := fresh x in rename x into x'; destruct H as [-> H] end.
     wp_pure. wp_apply wp_NewSlice. simpl. rewrite SessionPrelude.replicate_nil; cycle 1. { word. } iIntros "%s1 H_s1".
     wp_pures. wp_apply wp_ref_to. { repeat econstructor; eauto. } iIntros "%outGoingRequests H_outGoingRequests".
     wp_pures. wp_apply wp_ref_to. { repeat econstructor; eauto. } iIntros "%server H_server".
@@ -224,42 +224,42 @@ Section heap.
     { wp_apply wp_ref_to. { repeat econstructor; eauto. } iIntros "%succeeded H_succeeded".
       wp_pures. wp_apply wp_ref_to. { repeat econstructor; eauto. } iIntros "%reply H_reply".
       wp_pures. wp_load. replace (processClientRequest (#s .(Server.Id), (#s .(Server.NumberOfServers), (t4, (t3, (t2, (t1, (t0, (t, #()))))))))%V (#msg .(Message.MessageType), (#msg .(Message.C2S_Client_Id), (#msg .(Message.C2S_Server_Id), (#msg .(Message.C2S_Client_OperationType), (#msg .(Message.C2S_Client_Data), (t7, (#msg .(Message.S2S_Gossip_Sending_ServerId), (#msg .(Message.S2S_Gossip_Receiving_ServerId), (t6, (#msg .(Message.S2S_Gossip_Index), (#msg .(Message.S2S_Acknowledge_Gossip_Sending_ServerId), (#msg .(Message.S2S_Acknowledge_Gossip_Receiving_ServerId), (#msg .(Message.S2S_Acknowledge_Gossip_Index), (#msg .(Message.S2C_Client_OperationType), (#msg .(Message.S2C_Client_Data), (t5, (#msg .(Message.S2C_Server_Id), (#msg .(Message.S2C_Client_Number), #()))))))))))))))))))%V) with (processClientRequest (server_val (s .(Server.Id), s .(Server.NumberOfServers), t4, t3, t2, t1, t0, t)) (message_val (msg .(Message.MessageType), msg .(Message.C2S_Client_Id), msg .(Message.C2S_Server_Id), msg .(Message.C2S_Client_OperationType), msg .(Message.C2S_Client_Data), t7, msg .(Message.S2S_Gossip_Sending_ServerId), msg .(Message.S2S_Gossip_Receiving_ServerId), t6, msg .(Message.S2S_Gossip_Index), msg .(Message.S2S_Acknowledge_Gossip_Sending_ServerId), msg .(Message.S2S_Acknowledge_Gossip_Receiving_ServerId), msg .(Message.S2S_Acknowledge_Gossip_Index), msg .(Message.S2C_Client_OperationType), msg .(Message.S2C_Client_Data), t5, msg .(Message.S2C_Server_Id), msg .(Message.S2C_Client_Number)))) by f_equal.
-      wp_apply (wp_processClientRequest (OWN_UnsatisfiedRequests := true) with "[H3 H4 H6 H7 H8 H9 H16 H20 H27]"). { iFrame. simplNotation; subst. done. } iIntros "%b %ns %nm (-> & H_server' & H_message' & H_message & %H1_postcondition & %H2_postcondition & %H3_postcondition & %H4_postcondition)".
+      wp_apply (wp_processClientRequest (OWN_UnsatisfiedRequests := true) with "[H3 H4 H6 H7 H8 H9 H16 H20 H27]"). { iFrame. simplNotation; subst. done. } iIntros "%b %ns %nm (-> & H_server' & H_message' & H_message & %H_postcondition)". destruct H_postcondition as (H_postcondition & H7_postcondtion). destruct H_postcondition as [H1_postcondition H2_postcondition H3_postcondtion H4_postcondition [H5_postcondition H6_postcondtion]].
       wp_store. wp_store. wp_pures; lazymatch goal with [ |- envs_entails _ (wp ?s ?E (App ?k ?e)%E ?Q) ] => eapply (tac_wp_store_ty _ _ _ _ _ _ [AppRCtx k]%list); [repeat econstructor; eauto | tc_solve | let l := reply in iAssumptionCore | reflexivity | simpl] end.
       wp_pures. wp_load. wp_if_destruct.
       - wp_load. wp_load. replace message_val with (message_into_val .(to_val)) by reflexivity. wp_apply (wp_SliceAppend with "[$H_s1]"). iIntros "%s2 H_s2".
         wp_store. wp_load. wp_load. wp_pures. simpl. iModIntro. iApply "HΦ".
         unfold coq_processRequest; rewrite Heqb; replace (uint.nat (W64 0)) with 0%nat by reflexivity. destruct (coq_processClientRequest s msg) as [[succeeded_v s_v] reply_v] eqn: H_OBS; simpl in *.
         subst succeeded_v; simpl in *. iFrame. simpl. done.
-      - wp_load. wp_pures. iDestruct "H_server'" as "(%H1 & %H2 & H3 & H4 & %H5 & H6 & H7 & H8 & H9 & %H10)". rename H17 into H17'. iDestruct "H_message'" as "(%H11 & %H12 & %H13 & %H14 & %H15 & H16 & %H17 & %H18 & %H19 & H20 & %H21 & %H22 & %H23 & %H24 & %H25 & %H26 & H27 & %H28 & %H29 & %H30)". simplNotation; subst.
+      - wp_load. wp_pures. iDestruct "H_server'" as "(%H1' & %H2' & H3 & H4 & %H5' & H6 & H7 & H8 & H9 & %H10')". rename H17 into H17''. iDestruct "H_message'" as "(%H11' & %H12' & %H13' & %H14' & %H15' & H16 & %H17' & %H18' & %H19' & H20 & %H21' & %H22' & %H23' & %H24' & %H25' & %H26' & H27 & %H28' & %H29' & %H30')". simplNotation; subst.
         replace (#msg .(Message.MessageType), (#msg .(Message.C2S_Client_Id), (#msg .(Message.C2S_Server_Id), (#msg .(Message.C2S_Client_OperationType), (#msg .(Message.C2S_Client_Data), (t7, (#msg .(Message.S2S_Gossip_Sending_ServerId), (#msg .(Message.S2S_Gossip_Receiving_ServerId), (t6, (#msg .(Message.S2S_Gossip_Index), (#msg .(Message.S2S_Acknowledge_Gossip_Sending_ServerId), (#msg .(Message.S2S_Acknowledge_Gossip_Receiving_ServerId), (#msg .(Message.S2S_Acknowledge_Gossip_Index), (#msg .(Message.S2C_Client_OperationType), (#msg .(Message.S2C_Client_Data), (t5, (#msg .(Message.S2C_Server_Id), (#msg .(Message.S2C_Client_Number), #()))))))))))))))))))%V with (message_into_val .(to_val) (msg .(Message.MessageType), msg .(Message.C2S_Client_Id), msg .(Message.C2S_Server_Id), msg .(Message.C2S_Client_OperationType), msg .(Message.C2S_Client_Data), t7, msg .(Message.S2S_Gossip_Sending_ServerId), msg .(Message.S2S_Gossip_Receiving_ServerId), t6, msg .(Message.S2S_Gossip_Index), msg .(Message.S2S_Acknowledge_Gossip_Sending_ServerId), msg .(Message.S2S_Acknowledge_Gossip_Receiving_ServerId), msg .(Message.S2S_Acknowledge_Gossip_Index), msg .(Message.S2C_Client_OperationType), msg .(Message.S2C_Client_Data), t5, msg .(Message.S2C_Server_Id), msg .(Message.S2C_Client_Number))) by reflexivity.
         iDestruct "H3" as "(%ops1 & H3 & H_ops1)". wp_apply (wp_SliceAppend with "[$H3]"). iIntros "%s2 H_s2". wp_apply (wp_storeField_struct with "[H_server]"); auto. iIntros "H_server".
         wp_pures. wp_load. wp_load. wp_pures. iModIntro. red in ns, nm. simpl in ns, nm. replace (Φ (#ns.1.1.1.1.1.1.1, (#ns.1.1.1.1.1.1.2, (s2, (ns.1.1.1.1.2, (ns.1.1.1.2, (ns.1.1.2, (ns.1.2, (ns.2, #()))))))), s1)%V) with (Φ (server_val (ns.1.1.1.1.1.1.1, ns.1.1.1.1.1.1.2, s2, ns.1.1.1.1.2, ns.1.1.1.2, ns.1.1.2, ns.1.2, ns.2)%core, s1)%V) by reflexivity. iApply "HΦ".
         unfold coq_processRequest; rewrite Heqb; replace (uint.nat (W64 0)) with 0%nat by reflexivity. do 7 destruct ns as [ns ?]; simpl in *. do 17 destruct nm as [nm ?]; simpl in *. subst.
-        destruct (coq_processClientRequest s msg) as [[b s'] msg'] eqn: H_OBS; simpl in *. rewrite Heqb0; simpl. iFrame; simplNotation; simpl. iSplitR ""; try done. iSplit; try done; iPureIntro. destruct H1_postcondition as [? ? ? ?]; split; simpl; trivial.
+        destruct (coq_processClientRequest s msg) as [[b s'] msg'] eqn: H_OBS; simpl in *. rewrite Heqb0; simpl. iFrame; simplNotation; simpl. iSplitR ""; try done.
     }
     wp_if_destruct.
     { wp_load. replace (receiveGossip (#s .(Server.Id), (#s .(Server.NumberOfServers), (t4, (t3, (t2, (t1, (t0, (t, #()))))))))%V (#msg .(Message.MessageType), (#msg .(Message.C2S_Client_Id), (#msg .(Message.C2S_Server_Id), (#msg .(Message.C2S_Client_OperationType), (#msg .(Message.C2S_Client_Data), (t7, (#msg .(Message.S2S_Gossip_Sending_ServerId), (#msg .(Message.S2S_Gossip_Receiving_ServerId), (t6, (#msg .(Message.S2S_Gossip_Index), (#msg .(Message.S2S_Acknowledge_Gossip_Sending_ServerId), (#msg .(Message.S2S_Acknowledge_Gossip_Receiving_ServerId), (#msg .(Message.S2S_Acknowledge_Gossip_Index), (#msg .(Message.S2C_Client_OperationType), (#msg .(Message.S2C_Client_Data), (t5, (#msg .(Message.S2C_Server_Id), (#msg .(Message.S2C_Client_Number), #()))))))))))))))))))%V) with (receiveGossip (server_val (s .(Server.Id), s .(Server.NumberOfServers), t4, t3, t2, t1, t0, t)) (message_val( msg .(Message.MessageType), msg .(Message.C2S_Client_Id), msg .(Message.C2S_Server_Id), msg .(Message.C2S_Client_OperationType), msg .(Message.C2S_Client_Data), t7, msg .(Message.S2S_Gossip_Sending_ServerId), msg .(Message.S2S_Gossip_Receiving_ServerId), t6, msg .(Message.S2S_Gossip_Index), msg .(Message.S2S_Acknowledge_Gossip_Sending_ServerId), msg .(Message.S2S_Acknowledge_Gossip_Receiving_ServerId), msg .(Message.S2S_Acknowledge_Gossip_Index), msg .(Message.S2C_Client_OperationType), msg .(Message.S2C_Client_Data), t5, msg .(Message.S2C_Server_Id), msg .(Message.S2C_Client_Number)))) by f_equal.
-      wp_apply (wp_receiveGossip with "[H3 H4 H6 H7 H8 H9 H16 H20 H27]"). { iFrame. simplNotation; subst. done. } iIntros "%r (Hr & H_message & [%H1_sorted %H2_sorted] & [%H_ServerMyOperations %H_ServerId])".
-      wp_store. wp_load. wp_load. TypeVector.des r. replace (#(W64 2), (zero_val uint64T, (zero_val uint64T, (zero_val uint64T, (zero_val uint64T, (zero_val (slice.T uint64T), (zero_val uint64T, (zero_val uint64T, (zero_val (slice.T (slice.T uint64T * (uint64T * unitT)%ht)), (zero_val uint64T, (#r, (#msg .(Message.S2S_Gossip_Sending_ServerId), (#msg .(Message.S2S_Gossip_Index), (zero_val uint64T, (zero_val uint64T, (zero_val (slice.T uint64T), (zero_val uint64T, (zero_val uint64T, #()))))))))))))))))))%V with (message_into_val .(to_val) (W64 2, W64 0, W64 0, W64 0, W64 0, Slice.nil, W64 0, W64 0, Slice.nil, W64 0, r, msg .(Message.S2S_Gossip_Sending_ServerId), msg .(Message.S2S_Gossip_Index), W64 0, W64 0, Slice.nil, W64 0, W64 0)) by reflexivity.
-      wp_apply (wp_SliceAppend with "[$H_s1]"). iIntros "%s2 H_s2". wp_store. wp_pures. wp_apply (wp_ref_to); auto. iIntros "%i H_i". wp_apply (wp_ref_to). { repeat econstructor; eauto. } iIntros "%reply H_reply". wp_pures. wp_apply (wp_ref_to); auto. iIntros "%succeeded H_succeeded". wp_pures. simpl in *.
+      wp_apply (wp_receiveGossip with "[H3 H4 H6 H7 H8 H9 H16 H20 H27]"). { iFrame. simplNotation; subst. done. } iIntros "%r (Hr & H_message & %H_pure)". destruct H_pure as [H1_sorted H2_sorted (H_Id & H_NumberOfServers & H_UnsatisfiedRequests & H_MyOperations & H_GossipAcknowledgements)].
+      wp_store. wp_apply wp_ref_to; auto. iIntros "%i H_i". TypeVector.des r. replace (#(W64 2), (zero_val uint64T, (zero_val uint64T, (zero_val uint64T, (zero_val uint64T, (zero_val (slice.T uint64T), (zero_val uint64T, (zero_val uint64T, (zero_val (slice.T (slice.T uint64T * (uint64T * unitT)%ht)), (zero_val uint64T, (#r, (#msg .(Message.S2S_Gossip_Sending_ServerId), (#msg .(Message.S2S_Gossip_Index), (zero_val uint64T, (zero_val uint64T, (zero_val (slice.T uint64T), (zero_val uint64T, (zero_val uint64T, #()))))))))))))))))))%V with (message_into_val .(to_val) (W64 2, W64 0, W64 0, W64 0, W64 0, Slice.nil, W64 0, W64 0, Slice.nil, W64 0, r, msg .(Message.S2S_Gossip_Sending_ServerId), msg .(Message.S2S_Gossip_Index), W64 0, W64 0, Slice.nil, W64 0, W64 0)) by reflexivity.
+      wp_apply wp_ref_to. { repeat econstructor; eauto. } iIntros "%reply H_reply". wp_apply (wp_ref_to); auto. iIntros "%succeeded H_succeeded". wp_pures.
       rename r into Id, w into NumberOfServers, t13 into UnsatisfiedRequests, t12 into VectorClock, t11 into OperationsPerformed, t10 into MyOperations, t9 into PendingOperations, t8 into GossipAcknowledgements.
       set (focus := (coq_receiveGossip s msg).(Server.UnsatisfiedRequests)).
-      set (loop_init := (0%nat, (coq_receiveGossip s msg, [Message.mk 2 0 0 0 0 [] 0 0 [] 0 ((coq_receiveGossip s msg).(Server.Id)) (msg.(Message.S2S_Gossip_Sending_ServerId)) (msg.(Message.S2S_Gossip_Index)) 0 0 [] 0 0]))).
-      set (loop_step := λ acc : nat * (Server.t * list Message.t), λ element : Message.t,
-        let '(i, (s, outGoingRequests)) := acc in
+      set (loop_init := (0%nat, coq_receiveGossip s msg, @nil Message.t)).
+      set (loop_step := λ acc : nat * Server.t * list Message.t, λ element : Message.t,
+        let '(i, s, outGoingRequests) := acc in
         let '(succeeded, s, reply) := coq_processClientRequest s element in
         if succeeded then
           let UnsatisfiedRequests := coq_deleteAtIndexMessage s.(Server.UnsatisfiedRequests) i in
-          (i, (Server.mk s.(Server.Id) s.(Server.NumberOfServers) UnsatisfiedRequests s.(Server.VectorClock) s.(Server.OperationsPerformed) s.(Server.MyOperations) s.(Server.PendingOperations) s.(Server.GossipAcknowledgements), outGoingRequests ++ [reply]))
+          (i, Server.mk s.(Server.Id) s.(Server.NumberOfServers) UnsatisfiedRequests s.(Server.VectorClock) s.(Server.OperationsPerformed) s.(Server.MyOperations) s.(Server.PendingOperations) s.(Server.GossipAcknowledgements), outGoingRequests ++ [reply])
         else
-          ((i + 1)%nat, (s, outGoingRequests))
+          ((i + 1)%nat, s, outGoingRequests)
       ).
-      set (n := length s .(Server.VectorClock)). rename s into s0. iDestruct "Hr" as "(%H1 & %H2 & H3 & H4 & %H5 & H6 & H7 & H8 & H9 & %H10)"; simplNotation; simpl in *.
+      set (n := length s .(Server.VectorClock)). rename s into s0. iDestruct "Hr" as "(%H1' & %H2' & H3 & H4 & %H5' & H6 & H7 & H8 & H9 & %H10')"; simplNotation; simpl in *.
       wp_apply (wp_forBreak_cond
         ( λ continue, ∃ prevs : list Message.t, ∃ nexts : list Message.t, ∃ s : Server.t, ∃ msgs : list Message.t, ∃ out_going_requests : Slice.t, ∃ index : nat, ∃ msgv : tuple_of [u64,u64,u64,u64,u64,Slice.t,u64,u64,Slice.t,u64,u64,u64,u64,u64,u64,Slice.t,u64,u64], ∃ b : bool, ∃ Id : w64, ∃ NumberOfServers : w64, ∃ UnsatisfiedRequests : Slice.t, ∃ VectorClock : Slice.t, ∃ OperationsPerformed : Slice.t, ∃ MyOperations : Slice.t, ∃ PendingOperations : Slice.t, ∃ GossipAcknowledgements : Slice.t,
           ⌜focus = prevs ++ nexts⌝ ∗
-          ⌜(index, (s, msgs)) = fold_left loop_step prevs loop_init⌝ ∗
+          ⌜(index, s, msgs) = fold_left loop_step prevs loop_init⌝ ∗
           outGoingRequests ↦[(slice.T (uint64T * (uint64T * (uint64T * (uint64T * (uint64T * (slice.T uint64T * (uint64T * (uint64T * (slice.T (slice.T uint64T * (uint64T * unitT)) * (uint64T * (uint64T * (uint64T * (uint64T * (uint64T * (uint64T * (slice.T uint64T * (uint64T * (uint64T * unitT)))))))))))))))))))%ht] slice_val out_going_requests ∗
           i ↦[uint64T] #index ∗
           reply ↦[(uint64T * (uint64T * (uint64T * (uint64T * (uint64T * (slice.T uint64T * (uint64T * (uint64T * (slice.T (slice.T uint64T * (uint64T * unitT)) * (uint64T * (uint64T * (uint64T * (uint64T * (uint64T * (uint64T * (slice.T uint64T * (uint64T * (uint64T * unitT))))))))))))))))))%ht] message_val msgv ∗
@@ -272,7 +272,7 @@ Section heap.
           operation_slice PendingOperations s.(Server.PendingOperations) n ∗
           own_slice_small GossipAcknowledgements uint64T (DfracOwn 1) s.(Server.GossipAcknowledgements) ∗
           message_slice out_going_requests msgs n 0%nat ∗
-          ⌜SERVER_INVARIANT s⌝ ∗
+          ⌜SERVER_INVARIANT (fun _s => True) s⌝ ∗
           ⌜length s.(Server.UnsatisfiedRequests) = (index + length nexts)%nat⌝ ∗
           ⌜drop index s.(Server.UnsatisfiedRequests) = nexts⌝ ∗
           ⌜length s.(Server.VectorClock) = length s0.(Server.VectorClock)⌝ ∗
@@ -281,11 +281,12 @@ Section heap.
           ⌜Id = s.(Server.Id)⌝ ∗
           ⌜NumberOfServers = s.(Server.NumberOfServers)⌝ ∗
           ⌜length (coq_receiveGossip s0 msg).(Server.GossipAcknowledgements) = length s.(Server.GossipAcknowledgements)⌝ ∗
-          ⌜continue = false -> nexts = []⌝
+          ⌜continue = false -> nexts = []⌝ ∗
+          ⌜u64_le_CONSTANT s.(Server.Id) /\ u64_le_CONSTANT s.(Server.NumberOfServers) /\ Forall u64_le_CONSTANT s.(Server.VectorClock) /\ Forall u64_le_CONSTANT s .(Server.GossipAcknowledgements)⌝
         )%I
-      with "[] [H_outGoingRequests H_server H3 H4 H6 H7 H8 H9 H_message H_s2 H_i H_reply H_succeeded]").
-      { subst Id NumberOfServers. clear Φ UnsatisfiedRequests VectorClock OperationsPerformed MyOperations PendingOperations GossipAcknowledgements.
-        iIntros "%Φ". iModIntro. iIntros "(%prevs & %nexts & %s & %msgs & %out_going_requests & %index & %msgv & %b & %Id & %NumberOfServers & %UnsatisfiedRequests & %VectorClock & %OperationsPerformed & %MyOperations & %PendingOperations & %GossipAcknowledgements & %FOCUS & %LOOP & H_outGoingRequests & H_i & H_reply & H_succeeded & H_server & H_UnsatisfiedRequests & H_VectorClock & H_OperationsPerformed & H_MyOperations & H_PendingOperations & H_GossipAcknowledgements & H_out_going_requests & %H_server_invariant & %claim1 & %claim2 & %claim3 & %claim4 & %claim5 & %claim6 & %claim7 & %LENGTH_GossipAcknowledgements & %H_continue) HΦ". iDestruct "H_UnsatisfiedRequests" as "(%msgv1 & [H1_UnsatisfiedRequests H2_UnsatisfiedRequests] & H3_UnsatisfiedRequests)".
+      with "[] [H_outGoingRequests H_server H3 H4 H6 H7 H8 H9 H_message H_s1 H_i H_reply H_succeeded]").
+      { destruct H1' as [_Id H1']. destruct H2' as [_NumberOfServers H2']. subst Id NumberOfServers. clear Φ UnsatisfiedRequests VectorClock OperationsPerformed MyOperations PendingOperations GossipAcknowledgements.
+        iIntros "%Φ". iModIntro. iIntros "(%prevs & %nexts & %s & %msgs & %out_going_requests & %index & %msgv & %b & %Id & %NumberOfServers & %UnsatisfiedRequests & %VectorClock & %OperationsPerformed & %MyOperations & %PendingOperations & %GossipAcknowledgements & %FOCUS & %LOOP & H_outGoingRequests & H_i & H_reply & H_succeeded & H_server & H_UnsatisfiedRequests & H_VectorClock & H_OperationsPerformed & H_MyOperations & H_PendingOperations & H_GossipAcknowledgements & H_out_going_requests & %H_server_invariant & %claim1 & %claim2 & %claim3 & %claim4 & %claim5 & %claim6 & %claim7 & %LENGTH_GossipAcknowledgements & %H_continue & %H1_CONSTANT & %H2_CONSTANT & %H3_CONSTANT & %H4_CONSTANT) HΦ". iDestruct "H_UnsatisfiedRequests" as "(%msgv1 & [H1_UnsatisfiedRequests H2_UnsatisfiedRequests] & H3_UnsatisfiedRequests)".
         wp_load. wp_load. wp_apply (wp_slice_len). wp_if_destruct.
         - wp_pures. wp_load. wp_pures. wp_load. wp_pures.
           iPoseProof (big_sepL2_length with "[$H3_UnsatisfiedRequests]") as "%YES1".
@@ -301,12 +302,12 @@ Section heap.
           wp_apply (wp_SliceGet with "[$H1_UnsatisfiedRequests]"). { iPureIntro. exact H_e. } iIntros "H1_UnsatisfiedRequests".
           wp_load. wp_apply (wp_processClientRequest (OWN_UnsatisfiedRequests := false) with "[H_VectorClock H_OperationsPerformed H_MyOperations H_PendingOperations H_GossipAcknowledgements is_message_cur']").
           { iSplitR "is_message_cur'".
-            - iFrame; simplNotation; done.
+            - iFrame; simplNotation; try done.
             - iSplitL "is_message_cur'".
               + iExact "is_message_cur'".
-              + iPureIntro; done.
+              + destruct H_server_invariant. iPureIntro; split; eauto.
           }
-          iIntros "%r %ns %nm (-> & is_server_ns & is_message_nm & is_message_cur' & %H1_invariant & %H2_invariant & %H3_invariant & %H4_invariant)". wp_store. wp_store. wp_pures; lazymatch goal with [ |- envs_entails _ (wp ?s ?E (App ?k ?e)%E ?Q) ] => eapply (tac_wp_store_ty _ _ _ _ _ _ [AppRCtx k]%list); [repeat econstructor; eauto | tc_solve | let l := reply in iAssumptionCore | reflexivity | simpl] end. wp_load. wp_if_destruct.
+          iIntros "%r %ns %nm (-> & is_server_ns & is_message_nm & is_message_cur' & %H_pure)". destruct H_pure as [H_invariant H_pure]; simpl in *. destruct H_invariant. wp_store. wp_store. wp_pures; lazymatch goal with [ |- envs_entails _ (wp ?s ?E (App ?k ?e)%E ?Q) ] => eapply (tac_wp_store_ty _ _ _ _ _ _ [AppRCtx k]%list); [repeat econstructor; eauto | tc_solve | let l := reply in iAssumptionCore | reflexivity | simpl] end. wp_load. wp_if_destruct.
           + wp_load. wp_load. iDestruct "H_out_going_requests" as "(%ops1 & H_out_going_requests & H_ops1)". replace (message_val nm) with (message_into_val.(to_val) nm) by reflexivity. wp_apply (wp_SliceAppend with "[$H_out_going_requests]"). iIntros "%out_going_requests' H_out_goint_requests'".
             wp_store. wp_load. wp_load. wp_pures. TypeVector.des ns; simplNotation; subst t13. wp_apply (wp_deleteAtIndexMessage with "[$H1_UnsatisfiedRequests $H2_UnsatisfiedRequests message_slice_prevs' message_slice_nexts' is_message_cur']").
             { instantiate (1 := (prevs' ++ cur' :: nexts')%list). iSplitR "".
@@ -331,16 +332,16 @@ Section heap.
             iExists (prevs ++ [cur]). iExists nexts. iExists (let s : Server.t := (coq_processClientRequest s cur).1.2 in Server.mk s.(Server.Id) s.(Server.NumberOfServers) (coq_deleteAtIndexMessage s.(Server.UnsatisfiedRequests) index) s.(Server.VectorClock) s.(Server.OperationsPerformed) s.(Server.MyOperations) s.(Server.PendingOperations) s.(Server.GossipAcknowledgements)). iExists (msgs ++ [(coq_processClientRequest s cur).2])%list. iExists _. iExists index. iExists _. iExists _. iExists _. iExists _. iExists _. iExists _. iExists _. iExists _. iExists _. iExists _. iFrame.
             iSplitL "". { rewrite <- app_assoc. done. }
             iSplitL "". { iPureIntro. rewrite fold_left_app. simpl. rewrite <- LOOP. simpl. destruct (coq_processClientRequest s cur) as [[b' s'] reply']; simpl in *. subst b'. replace (uint.nat (W64 index)) with index by word. reflexivity. }
-            iSplitL "message_slice_ns2". { simpl. rewrite <- EQ. replace (uint.nat (W64 index)) with index by word. rewrite <- H2_invariant. iExact "message_slice_ns2". }
-            simpl in *. iDestruct "is_server_ns" as "(%H1'' & %H2'' & H3'' & H4'' & %H5'' & H6'' & H7'' & H8'' & H9'' & %H10'')". iFrame. iPureIntro.
-            simplNotation; subst; simpl; split. { destruct H1_invariant. split; simpl; trivial. } rewrite <- EQ in LEN_ns2. replace (uint.nat (W64 (length prevs'))) with (length prevs') in * by word. repeat (split; try done).
-            * rewrite <- H2_invariant. word.
-            * unfold coq_deleteAtIndexMessage. rewrite <- H2_invariant. rewrite <- drop_drop. replace (uint.nat (W64 (length prevs'))) with (length prevs') in * by word. rewrite -> claim2. simpl. replace (drop 0 nexts) with nexts by reflexivity. rewrite drop_app.
-              replace (drop (length prevs') (take (length prevs') s .(Server.UnsatisfiedRequests))) with ( @nil Message.t) by now symmetry; eapply nil_length_inv; rewrite length_drop; rewrite length_take; word.
-              replace (length prevs' - length (take (length prevs') s .(Server.UnsatisfiedRequests)))%nat with 0%nat by now rewrite length_take; word.
-              reflexivity.
+            iSplitL "message_slice_ns2". { simpl. rewrite <- EQ. replace (uint.nat (W64 index)) with index by word. destruct EXTRA_SERVER_INVARIANT0 as [H2_invariant H1_invariant]. rewrite -> H2_invariant. rewrite <- EQ. iExact "message_slice_ns2". }
+            simpl in *. iDestruct "is_server_ns" as "(%H1'' & %H2'' & H3'' & H4'' & %H5'' & H6'' & H7'' & H8'' & H9'' & %H10'')". iFrame. iPureIntro. simplNotation; repeat match goal with [ H : ?x = _ /\ _ |- _ ] => destruct H as [? H]; try subst x end.
+            subst; simpl; split. { split; simpl; trivial. } rewrite <- EQ in LEN_ns2. replace (uint.nat (W64 (length prevs'))) with (length prevs') in * by word. repeat (split; try done).
+            * rewrite H3. rewrite <- EQ. word. 
+            * unfold coq_deleteAtIndexMessage. rewrite H3.
+              replace (take (length prevs') (prevs' ++ cur :: nexts)) with (take (length prevs') (prevs' ++ nexts)); cycle 1. { symmetry. rewrite -> take_app. rewrite -> take_app. replace (length prevs' - length prevs')%nat with 0%nat by word. reflexivity. }
+              replace (drop (length prevs' + 1) (prevs' ++ cur :: nexts)) with (drop (length prevs') (prevs' ++ nexts)); cycle 1. { symmetry. rewrite <- drop_drop. rewrite drop_app_length. rewrite drop_app_length. reflexivity. }
+              rewrite take_drop. rewrite drop_app_length; trivial.
             * word.
-            * rewrite <- H2_invariant. word.
+            * rewrite H3. rewrite <- ns2_SZ. congruence.
           + TypeVector.des ns; simplNotation; subst t13.
             assert (length prevs' = index) as claim8 by word.
             assert (cur = cur' /\ nexts = nexts') as [<- <-].
@@ -354,13 +355,14 @@ Section heap.
             iExists (prevs ++ [cur])%list. iExists nexts. iExists ((coq_processClientRequest s cur).1.2). iExists msgs. iExists _. iExists (index + 1)%nat. iExists _. iExists _. iExists _. iExists _. iExists _. iExists _. iExists _. iExists _. iExists _. iExists _. replace (w64_word_instance .(word.add) (W64 index) (W64 1)) with (W64 (index + 1)%nat) by word. iFrame.
             iSplitL "". { rewrite <- app_assoc. done. }
             iSplitL "". { iPureIntro. rewrite fold_left_app. simpl. rewrite <- LOOP. simpl. destruct (coq_processClientRequest s cur) as [[b' s'] reply']; simpl in *. subst b'; reflexivity. }
-            iSplitL "message_slice_prevs' message_slice_nexts' is_message_cur'". { replace (uint.nat (W64 index)) with index in H_e |- * by word. rewrite <- H2_invariant, -> EQ. iApply (big_sepL2_middle_merge with "[is_message_cur' $message_slice_prevs' $message_slice_nexts']"); eauto. }
+            iSplitL "message_slice_prevs' message_slice_nexts' is_message_cur'". { replace (uint.nat (W64 index)) with index in H_e |- * by word. destruct EXTRA_SERVER_INVARIANT0 as [H2_invariant H1_invariant]. rewrite -> H2_invariant. iApply (big_sepL2_middle_merge with "[is_message_cur' $message_slice_prevs' $message_slice_nexts']"); eauto. }
             simpl in *. iDestruct "is_server_ns" as "(%H1'' & %H2'' & H3'' & H4'' & %H5'' & H6'' & H7'' & H8'' & H9'' & %H10'')". iFrame. iPureIntro.
-            simplNotation; subst; simpl; split. { destruct H1_invariant. split; simpl; trivial. } repeat (split; try done).
-            * rewrite <- H2_invariant. apply f_equal with (f := length) in EQ. rewrite length_app in EQ. simpl in *. word.
-            * rewrite <- drop_drop. rewrite <- H2_invariant. rewrite -> claim2. simpl. replace (drop 0 nexts) with nexts by reflexivity. reflexivity.
+            simplNotation; subst; simpl; split. { split; simpl; trivial. } repeat (split; try done); try tauto.
+            * rewrite -? H2_invariant. apply f_equal with (f := length) in EQ. rewrite length_app in EQ. simpl in *. destruct EXTRA_SERVER_INVARIANT0 as [EQ1 EQ2]. rewrite EQ1. rewrite length_app; simpl; word.
+            * rewrite <- drop_drop. destruct EXTRA_SERVER_INVARIANT0 as [EQ1 EQ2]. rewrite EQ1. rewrite drop_app_length; trivial.
             * word.
-            * rewrite <- H2_invariant. word.
+            * word.
+            * destruct EXTRA_SERVER_INVARIANT0 as [EQ1 EQ2]. rewrite EQ1. rewrite <- EQ. word.
         - iModIntro. iApply "HΦ".
           iExists prevs. iExists nexts. iExists s. iExists msgs. iExists _. iExists index. iExists _. iExists _. iExists _. iExists _. iExists _. iExists _. iExists _. iExists _. iExists _. iExists _. iFrame. iPureIntro.
           simplNotation; subst; simpl; split. { trivial. } repeat (split; try done). intros _.
@@ -368,48 +370,21 @@ Section heap.
       }
       { iAssert ⌜length (coq_receiveGossip s0 msg) .(Server.UnsatisfiedRequests) = uint.nat UnsatisfiedRequests .(Slice.sz)⌝%I as "%UnsatisfiedRequests_SZ".
         { iDestruct "H3" as "(%ops1 & H3 & Hops1)". iPoseProof (big_sepL2_length with "[$Hops1]") as "%LEN1". iPoseProof (own_slice_sz with "[$H3]") as "%LEN2". word. }
-        iExists []. iExists focus. iExists (coq_receiveGossip s0 msg). iExists [Message.mk 2 0 0 0 0 [] 0 0 [] 0 ((coq_receiveGossip s0 msg).(Server.Id)) (msg.(Message.S2S_Gossip_Sending_ServerId)) (msg.(Message.S2S_Gossip_Index)) 0 0 [] 0 0]. iExists s2. iExists 0%nat. iExists (W64 0, W64 0, W64 0, W64 0, W64 0, Slice.nil, W64 0, W64 0, Slice.nil, W64 0, W64 0, W64 0, W64 0, W64 0, W64 0, Slice.nil, W64 0, W64 0). iExists false. iExists Id. iExists NumberOfServers. iExists UnsatisfiedRequests. iExists VectorClock. iExists OperationsPerformed. iExists MyOperations. iExists PendingOperations. iExists GossipAcknowledgements. iFrame.
+        iExists []. iExists focus. iExists (coq_receiveGossip s0 msg). iExists []. iExists s1. iExists 0%nat. iExists (W64 0, W64 0, W64 0, W64 0, W64 0, Slice.nil, W64 0, W64 0, Slice.nil, W64 0, W64 0, W64 0, W64 0, W64 0, W64 0, Slice.nil, W64 0, W64 0). iExists false. iExists Id. iExists NumberOfServers. iExists UnsatisfiedRequests. iExists VectorClock. iExists OperationsPerformed. iExists MyOperations. iExists PendingOperations. iExists GossipAcknowledgements.
+        simplNotation; repeat match goal with [ H : ?x = _ /\ _ |- _ ] => destruct H as [? H]; try subst x end. subst n. rewrite <- H3. iFrame.
         iSplitL "". { done. }
         iSplitL "". { simpl. done. }
-        iSplitL "".
-        { simpl. iSplitR ""; eauto. iExists 0%nat. repeat (iSplit; try done); simplNotation.
-          iSplitL "". { iApply own_slice_small_nil; eauto. }
-          iSplitL "". { done. }
-          iSplitL "". { done. }
-          iSplitL "". { done. }
-          iSplitL "". { iExists []; iSplit; simpl; try done; iApply own_slice_nil; eauto. }
-          iSplitL "". { done. }
-          iSplitL "". { done. }
-          iSplitL "". { done. }
-          iSplitL "". { done. }
-          iSplitL "". { done. }
-          iSplitL "". { done. }
-          iSplitL "". { iApply own_slice_small_nil; eauto. }
-          done.
-        }
-        iPureIntro. split.
-        { split; trivial.
-          - rewrite <- H_ServerMyOperations; trivial.
-          - rewrite <- H_ServerId; word.
-        }
-        split. { unfold focus. word. }
-        split. { unfold focus. reflexivity. }
-        split. { word. }
-        split. { word. }
-        split. { eauto. }
-        split. { word. }
-        split. { word. }
-        split. { word. }
-        congruence.
+        iSplitL "". { simpl. done. }
+        iPureIntro. repeat (split; (word || tauto || trivial)). rewrite H_MyOperations; trivial.
       }
-      { subst. clear UnsatisfiedRequests VectorClock OperationsPerformed MyOperations PendingOperations GossipAcknowledgements. iIntros "(%prevs & %nexts & %s & %msgs & %out_going_requests & %index & %msgv & %b & %Id & %NumberOfServers & %UnsatisfiedRequests & %VectorClock & %OperationsPerformed & %MyOperations & %PendingOperations & %GossipAcknowledgements & %FOCUS & %LOOP & H_outGoingRequests & H_i & H_reply & H_succeeded & H_server & H_UnsatisfiedRequests & H_VectorClock & H_OperationsPerformed & H_MyOperations & H_PendingOperations & H_GossipAcknowledgements & H_out_going_requests & %H_server_invariant & %claim1 & %claim2 & %claim3 & %claim4 & %claim5 & %claim6 & %claim7 & %LENGTH_GossipAcknowledgements & %H_continue)". iDestruct "H_UnsatisfiedRequests" as "(%msgv1 & [H1_UnsatisfiedRequests H2_UnsatisfiedRequests] & H3_UnsatisfiedRequests)".
+      { repeat match goal with [ H : ?x = _ /\ _ |- _ ] => destruct H as [? H]; try subst x end. subst. clear UnsatisfiedRequests VectorClock OperationsPerformed MyOperations PendingOperations GossipAcknowledgements. iIntros "(%prevs & %nexts & %s & %msgs & %out_going_requests & %index & %msgv & %b & %Id & %NumberOfServers & %UnsatisfiedRequests & %VectorClock & %OperationsPerformed & %MyOperations & %PendingOperations & %GossipAcknowledgements & %FOCUS & %LOOP & H_outGoingRequests & H_i & H_reply & H_succeeded & H_server & H_UnsatisfiedRequests & H_VectorClock & H_OperationsPerformed & H_MyOperations & H_PendingOperations & H_GossipAcknowledgements & H_out_going_requests & %H_server_invariant & %claim1 & %claim2 & %claim3 & %claim4 & %claim5 & %claim6 & %claim7 & %LENGTH_GossipAcknowledgements & %H_continue & %H_pure)". iDestruct "H_UnsatisfiedRequests" as "(%msgv1 & [H1_UnsatisfiedRequests H2_UnsatisfiedRequests] & H3_UnsatisfiedRequests)".
         specialize (H_continue eq_refl). subst nexts. rewrite H_continue in FOCUS. rewrite app_nil_r in FOCUS. subst prevs.
         wp_load. wp_load. wp_pures. iModIntro. iApply "HΦ".
         iSplitL "H1_UnsatisfiedRequests H2_UnsatisfiedRequests H3_UnsatisfiedRequests H_VectorClock H_OperationsPerformed H_MyOperations H_PendingOperations H_GossipAcknowledgements".
-        { iFrame; simplNotation; subst; iFrame. unfold coq_processRequest; rewrite Heqb0; replace (uint.nat (W64 1)) with 1%nat by word; simpl; fold loop_step; fold loop_init; fold focus; rewrite <- LOOP; simpl; iFrame.
-          iPureIntro; repeat (split; try done). rewrite H10; trivial.
+        { iFrame; simplNotation; subst; iFrame. unfold coq_processRequest. rewrite Heqb0. replace (uint.nat (W64 1)) with 1%nat by word. simpl; fold loop_init. fold loop_step; fold focus. rewrite <- LOOP; simpl. subst n. rewrite H3. iFrame.
+          iPureIntro; repeat (split; word || tauto || done || trivial).
         } 
-        unfold coq_processRequest; rewrite Heqb0; replace (uint.nat (W64 1)) with 1%nat by word; simpl; fold loop_step; fold loop_init; fold focus; rewrite <- LOOP; simpl; iFrame. done.
+        unfold coq_processRequest; rewrite Heqb0; replace (uint.nat (W64 1)) with 1%nat by word; simpl; fold loop_step; fold loop_init; fold focus; rewrite <- LOOP; simpl; iFrame. subst n. rewrite H3. iSplitR ""; done.
       }
     }
     wp_if_destruct.
@@ -417,50 +392,54 @@ Section heap.
       wp_apply (wp_acknowledgeGossip (OWN_UnsatisfiedRequests := true) with "[H3 H4 H6 H7 H8 H9 H16 H20 H27]"). { iFrame; simplNotation; simpl. done. } iIntros "[H_is_server H_is_message]". wp_store. wp_load. wp_load. wp_pures.
       iModIntro. iApply "HΦ". unfold coq_processRequest; rewrite Heqb1; replace (uint.nat (W64 2)) with 2%nat by word; simpl; iFrame. iSplitR "".
       - simpl; done.
-      - iPureIntro; unfold coq_acknowledgeGossip. destruct (uint.Z msg .(Message.S2S_Acknowledge_Gossip_Sending_ServerId) >=? length s .(Server.GossipAcknowledgements)) as [ | ] eqn: H_OBS; split; trivial.
+      - iPureIntro; unfold coq_acknowledgeGossip. destruct (uint.nat msg .(Message.S2S_Acknowledge_Gossip_Sending_ServerId) >=? length s .(Server.GossipAcknowledgements)) as [ | ] eqn: H_OBS; split; trivial; simpl.
     }
     wp_if_destruct.
-    { wp_apply (wp_ref_to); auto. iIntros "%i H_i". wp_pures.
-      set (loop_init := @nil Message.t).
-      set (loop_step := λ acc : list Message.t, λ index : u64,
-        if negb (uint.nat index =? uint.nat s.(Server.Id))%nat && negb (length (coq_getGossipOperations s index) =? 0)%nat then
-          let S2S_Gossip_Sending_ServerId := s.(Server.Id) in
+    { admit. (* wp_apply (wp_ref_to); auto. iIntros "%i H_i". wp_pures.
+      set (loop_init := (s, @nil Message.t)).
+      set (loop_step := λ acc : Server.t * list Message.t, λ index : u64,
+        let '(server, outGoingRequests) := acc in
+        if negb (uint.nat index =? uint.nat server.(Server.Id))%nat && negb (length (coq_getGossipOperations server index) =? 0)%nat then
+          let GossipAcknowledgements := <[uint.nat index := W64 (length server.(Server.MyOperations))]> server.(Server.GossipAcknowledgements) in
+          let S2S_Gossip_Sending_ServerId := server.(Server.Id) in
           let S2S_Gossip_Receiving_ServerId := index in
-          let S2S_Gossip_Operations := coq_getGossipOperations s index in
-          let S2S_Gossip_Index := length (s.(Server.MyOperations)) in
+          let S2S_Gossip_Operations := coq_getGossipOperations server index in
+          let S2S_Gossip_Index := length (server.(Server.MyOperations)) in
           let message := Message.mk 1 0 0 0 0 [] S2S_Gossip_Sending_ServerId S2S_Gossip_Receiving_ServerId S2S_Gossip_Operations S2S_Gossip_Index 0 0 0 0 0 [] 0 0 in
-          acc ++ [message]
+          (Server.mk server.(Server.Id) server.(Server.NumberOfServers) server.(Server.UnsatisfiedRequests) server.(Server.VectorClock) server.(Server.OperationsPerformed) server.(Server.MyOperations) server.(Server.PendingOperations) GossipAcknowledgements, outGoingRequests ++ [message])
         else
-          acc
+          (server, outGoingRequests)
       ).
       iAssert ⌜uint.nat t1.(Slice.sz) = length s .(Server.MyOperations)⌝%I as "%t1_SZ".
       { iDestruct "H7" as "(%ops1 & H7 & H_ops1)". iPoseProof (big_sepL2_length with "[$H_ops1]") as "%LEN1". iPoseProof (own_slice_sz with "[$H7]") as "%LEN2". word. }
       wp_apply (wp_forBreak_cond
-        ( λ continue, ∃ index : nat, ∃ msgs : list Message.t, ∃ out_going_requests : Slice.t,
-          ⌜msgs = fold_left loop_step (map (λ i : nat, W64 i) (seq 0%nat index)) loop_init⌝ ∗
+        ( λ continue, ∃ s' : Server.t, ∃ GossipAcknowledgements' : Slice.t, ∃ index : nat, ∃ msgs : list Message.t, ∃ out_going_requests : Slice.t,
+          ⌜(s', msgs) = fold_left loop_step (map (λ i : nat, W64 i) (seq 0%nat index)) loop_init⌝ ∗
           i ↦[uint64T] #(W64 index) ∗
-          server ↦[(uint64T * (uint64T * (slice.T (uint64T * (uint64T * (uint64T * (uint64T * (uint64T * (slice.T uint64T * (uint64T * (uint64T * (slice.T (slice.T uint64T * (uint64T * unitT)) * (uint64T * (uint64T * (uint64T * (uint64T * (uint64T * (uint64T * (slice.T uint64T * (uint64T * (uint64T * unitT)))))))))))))))))) * (slice.T uint64T * (slice.T (slice.T uint64T * (uint64T * unitT)) * (slice.T (slice.T uint64T * (uint64T * unitT)) * (slice.T (slice.T uint64T * (uint64T * unitT)) * (slice.T uint64T * unitT))))))))%ht] server_val (s.(Server.Id), s.(Server.NumberOfServers), t4, t3, t2, t1, t0, t)%core ∗
+          server ↦[(uint64T * (uint64T * (slice.T (uint64T * (uint64T * (uint64T * (uint64T * (uint64T * (slice.T uint64T * (uint64T * (uint64T * (slice.T (slice.T uint64T * (uint64T * unitT)) * (uint64T * (uint64T * (uint64T * (uint64T * (uint64T * (uint64T * (slice.T uint64T * (uint64T * (uint64T * unitT)))))))))))))))))) * (slice.T uint64T * (slice.T (slice.T uint64T * (uint64T * unitT)) * (slice.T (slice.T uint64T * (uint64T * unitT)) * (slice.T (slice.T uint64T * (uint64T * unitT)) * (slice.T uint64T * unitT))))))))%ht] server_val (s'.(Server.Id), s'.(Server.NumberOfServers), t4, t3, t2, t1, t0, t)%core ∗
           outGoingRequests ↦[(slice.T (uint64T * (uint64T * (uint64T * (uint64T * (uint64T * (slice.T uint64T * (uint64T * (uint64T * (slice.T (slice.T uint64T * (uint64T * unitT)) * (uint64T * (uint64T * (uint64T * (uint64T * (uint64T * (uint64T * (slice.T uint64T * (uint64T * (uint64T * unitT)))))))))))))))))))%ht] slice_val out_going_requests ∗
-          message_slice t4 s .(Server.UnsatisfiedRequests) (length s .(Server.VectorClock)) (length s .(Server.VectorClock)) ∗
+          message_slice t4 s .(Server.UnsatisfiedRequests) (length s'.(Server.VectorClock)) (length s'.(Server.VectorClock)) ∗
           own_slice_small t3 uint64T (DfracOwn 1) s .(Server.VectorClock) ∗
-          operation_slice t2 s .(Server.OperationsPerformed) (length s .(Server.VectorClock)) ∗
-          operation_slice t1 s .(Server.MyOperations) (length s .(Server.VectorClock)) ∗
-          operation_slice t0 s .(Server.PendingOperations) (length s .(Server.VectorClock)) ∗
-          own_slice_small t uint64T (DfracOwn 1) s .(Server.GossipAcknowledgements) ∗
+          operation_slice t2 s .(Server.OperationsPerformed) (length s'.(Server.VectorClock)) ∗
+          operation_slice t1 s .(Server.MyOperations) (length s'.(Server.VectorClock)) ∗
+          operation_slice t0 s .(Server.PendingOperations) (length s'.(Server.VectorClock)) ∗
+          own_slice_small GossipAcknowledgements' uint64T (DfracOwn 1) s'.(Server.GossipAcknowledgements) ∗
           own_slice_small t7 uint64T (DfracOwn 1) msg .(Message.C2S_Client_VersionVector) ∗
-          operation_slice t6 msg .(Message.S2S_Gossip_Operations) (length s .(Server.VectorClock)) ∗
+          operation_slice t6 msg .(Message.S2S_Gossip_Operations) (length s'.(Server.VectorClock)) ∗
           own_slice_small t5 uint64T (DfracOwn 1) msg .(Message.S2C_Client_VersionVector) ∗
-          message_slice out_going_requests msgs (length s .(Server.VectorClock)) 0%nat ∗
-          ⌜index = uint.nat (W64 index) /\ uint.Z (W64 index) ≤ uint.Z s .(Server.NumberOfServers)⌝ ∗
-          ⌜continue = false -> index = uint.nat s.(Server.NumberOfServers)⌝
+          message_slice out_going_requests msgs (length s'.(Server.VectorClock)) 0%nat ∗
+          ⌜index = uint.nat (W64 index) /\ uint.Z (W64 index) ≤ uint.Z s'.(Server.NumberOfServers)⌝ ∗
+          ⌜continue = false -> index = uint.nat s'.(Server.NumberOfServers)⌝ ∗
+          ⌜SERVER_INVARIANT (fun _s => True) s' /\ Z.of_nat (length s'.(MyOperations)) <= CONSTANT⌝
         )%I
       with "[] [H3 H4 H6 H7 H8 H9 H16 H20 H27 H_i H_server H_outGoingRequests H_s1]").
-      { clear Φ. iIntros "%Φ". iModIntro. iIntros "(%index & %msgs & %out_going_requests & %H_msgs & H_i & H_server & H_outGoingRequests & H_UnsatisfiedRequests & H_VectorClock & H_OperationsPerformed & H_MyOperations & H_PendingOperations &H_GossipAcknowledgements & H_C2S_Client_VersionVector & H_S2S_Gossip_Operations & H_S2C_Client_VersionVector & H_out_going_requests & [%i_BOUND %i_BOUND'] & %H_continue) HΦ".
+      { clear Φ. iIntros "%Φ". iModIntro. iIntros "(%s' & %GossipAcknowledgements' & %index & %msgs & %out_going_requests & %H_msgs & H_i & H_server & H_outGoingRequests & H_UnsatisfiedRequests & H_VectorClock & H_OperationsPerformed & H_MyOperations & H_PendingOperations &H_GossipAcknowledgements & H_C2S_Client_VersionVector & H_S2S_Gossip_Operations & H_S2C_Client_VersionVector & H_out_going_requests & [%i_BOUND %i_BOUND'] & %H_continue) HΦ".
+        Print SERVER_INVARIANT.
         wp_load. wp_if_destruct.
         - wp_load. wp_load. wp_if_destruct.
-          + wp_load. wp_load. wp_apply (wp_getGossipOperations (OWN_UnsatisfiedRequests := true) with "[H_UnsatisfiedRequests H_VectorClock H_OperationsPerformed H_MyOperations H_PendingOperations H_GossipAcknowledgements]"). { iFrame; simplNotation; simpl; done. } iIntros "%ns [H_ns H_is_server]".
+          + wp_load. wp_load. wp_apply (wp_getGossipOperations (OWN_UnsatisfiedRequests := true) with "[H_UnsatisfiedRequests H_VectorClock H_OperationsPerformed H_MyOperations H_PendingOperations H_GossipAcknowledgements]"). { iFrame; simplNotation; simpl. iPureIntro; repeat (split; (word || tauto || done || trivial)). } iIntros "%ns [H_ns H_is_server]".
             replace (coq_getGossipOperations s (uint.nat (W64 index))) with (coq_getGossipOperations s index) in * by now f_equal; word. wp_apply wp_slice_len. wp_if_destruct.
-            * wp_load. wp_load. wp_pures. wp_apply wp_slice_len. wp_load. refine (let TMP : w64 := t1 .(Slice.sz) in _). fold TMP. replace (#(W64 1), (zero_val uint64T, (zero_val uint64T, (zero_val uint64T, (zero_val uint64T, (zero_val (slice.T uint64T), (#s .(Server.Id), (#(W64 index), (ns, (#TMP, (zero_val uint64T, (zero_val uint64T, (zero_val uint64T, (zero_val uint64T, (zero_val uint64T, (zero_val (slice.T uint64T), (zero_val uint64T, (zero_val uint64T, #()))))))))))))))))))%V with (message_into_val .(to_val) (W64 1, W64 0, W64 0, W64 0, W64 0, Slice.nil, s.(Server.Id), (W64 index), ns, TMP, W64 0, W64 0, W64 0, W64 0, W64 0, Slice.nil, W64 0, W64 0)) by reflexivity. subst TMP.
+            * wp_load. wp_pures. wp_apply wp_SliceSet. wp_load. wp_pures. wp_apply wp_slice_len. wp_load. refine (let TMP : w64 := t1 .(Slice.sz) in _). fold TMP. replace (#(W64 1), (zero_val uint64T, (zero_val uint64T, (zero_val uint64T, (zero_val uint64T, (zero_val (slice.T uint64T), (#s .(Server.Id), (#(W64 index), (ns, (#TMP, (zero_val uint64T, (zero_val uint64T, (zero_val uint64T, (zero_val uint64T, (zero_val uint64T, (zero_val (slice.T uint64T), (zero_val uint64T, (zero_val uint64T, #()))))))))))))))))))%V with (message_into_val .(to_val) (W64 1, W64 0, W64 0, W64 0, W64 0, Slice.nil, s.(Server.Id), (W64 index), ns, TMP, W64 0, W64 0, W64 0, W64 0, W64 0, Slice.nil, W64 0, W64 0)) by reflexivity. subst TMP.
               iDestruct "H_out_going_requests" as "(%msgv & H_out_going_requests & H_msgv)". wp_apply (wp_SliceAppend with "[$H_out_going_requests]"). iIntros "%out_going_requests' H_out_going_requests'". wp_store. wp_load. wp_store.
               iAssert ⌜uint.nat ns.(Slice.sz) = length (coq_getGossipOperations s index)⌝%I as "%ns_SZ".
               { iDestruct "H_ns" as "(%ops1 & H_ns & H_ops1)". iPoseProof (big_sepL2_length with "[$H_ops1]") as "%LEN1". iPoseProof (own_slice_sz with "[$H_ns]") as "%LEN2". word. }
@@ -531,7 +510,7 @@ Section heap.
         specialize (H_continue eq_refl). subst index msgs.
         iModIntro. iApply "HΦ".
         unfold coq_processRequest; replace (uint.nat msg.(Message.MessageType)) with 3%nat by word; simpl; fold loop_step; fold loop_init. iFrame; simplNotation; simpl. done.
-      }
+      } *)
     }
     { set (ns := (s.(Server.Id), s.(Server.NumberOfServers), t4, t3, t2, t1, t0, t)). replace (#s .(Server.Id), (#s .(Server.NumberOfServers), (t4, (t3, (t2, (t1, (t0, (t, #()))))))))%V with (server_val ns) by reflexivity.
       wp_load. wp_load. wp_pures. iModIntro.
@@ -540,7 +519,7 @@ Section heap.
       - split; try done.
       - split; trivial. split; trivial.
     }
-  Qed. *) Admitted.
+  Admitted.
 
   #[local] Opaque CoqSessionServer.processRequest.
 
